\documentclass[14pt]{extarticle}
\begin{document}
	\paragraph{Question/Claim} Prove that for any natural number n,
	\begin{equation}\label{eq:0}
	\sum\limits_{i=1}^n 2^i = 2+2^2+2^3+ ... +2^n=2^{n+1} - 2
	\end{equation}
	\paragraph{Proof} By mathematical induction.
	\paragraph{Initial Step} For $n=1$, the identity (\ref{eq:0}) reduces to:
	\begin{center}
		$2 = 2^{1+1}-2 = 4 - 2 = 2$
	\end{center}
	which is true since both sides are equal to 2. 
	\paragraph{Inductive Step} Assume identity (\ref{eq:0}) is true for $n$:
	\begin{equation}\label{eq:1}
	\sum\limits_{i=1}^n 2^i =  2^{n+1} - 2 
	\end{equation}
	Add $2^{n+1}$ to both sides of (\ref{eq:1}):
	\begin{equation}\label{eq:2}
		2^{n+1} + \sum\limits_{i=1}^n 2^i = 2^{n+1} + 2^{n+1} - 2
	\end{equation}
	By definition of summation and algebra, (\ref{eq:2}) reduces to:
	\begin{center}
		$\sum\limits_{i=1}^{n+1} 2^i = 2*2^{n+1} - 2 = 2^{(n+1)+1}-2$		
	\end{center}
	Which is identity (\ref{eq:0}) with $n+1$ in place of $n$.  Hence by the principle of mathematical induction, the identity holds for all $n \in \mathcal{N}$.
\end{document}